rocq-brick-libstdcpp/test/mutex/custom_recursive_mutex_hpp_proof.v
@@ -2,22 +2,11 @@
 
 Require Import skylabs.auto.cpp.proof.
 Require Import skylabs.brick.libstdcpp.mutex.spec.mutex.
-Require Import skylabs.brick.libstdcpp.mutex.spec.recursive_mutex.
+Require Import skylabs.brick.libstdcpp.mutex.spec.recursive_mutex_atomic.
 Require Import skylabs.brick.libstdcpp.test.mutex.custom_recursive_mutex_hpp.
-(*
-TODO step 1:
 
-split recursive_mutex specs:
-
-* C++- independent predicates vs
-* what's bound to C++ names
-
-* step2
-specs for atomic
-
-* step3???
-
- *)
+(** FIXME don't need StdAtomicSpecs *)
+Module StdAtomicSpecs := RecursiveMutexAtomicSpecs StdRecursiveMutexName.
 Module custom_recursive_mutex.
   Abbreviation N := "MyRecursiveMutex"%cpp_name.
 
@@ -32,10 +21,10 @@ Module custom_recursive_mutex.
   Parameter exclusive_token : ∀ `{Σ : cpp_logic}, iprop.gname -> mpred.
 
   Record gname : Set := MkGname
-  { lock_gname : iprop.gname
+  { lock_gname : mutex.gname
   ; cinv_gname : iprop.gname
   ; excl_gname : iprop.gname
-  ; rec_gname : recursive_mutex.gname
+  ; rec_gname : StdAtomicSpecs.gname
   }.
 
   Definition lock_namespace : namespace := nroot .@@ "MyRecursiveMutex".
@@ -43,15 +32,16 @@ Module custom_recursive_mutex.
   Parameter count_auth : ∀ `{Σ : cpp_logic} (count : nat), mpred.
   Parameter count_frag : ∀ `{Σ : cpp_logic} (count : nat), mpred.
 
-  (* Definition IR `{Σ : cpp_logic, σ : genv, !HasStdThreads Σ, !recursive_mutex.lockedG Σ} (γ : gname) (q : cQp.t) : mpred :=
-    ∃ x, recursive_mutex.owned_count_id_auth γ.(rec_gname) x. *)
+  (* Definition IR `{Σ : cpp_logic, σ : genv, !HasStdThreads Σ, !StdAtomicSpecs.lockedG Σ} (γ : gname) (q : cQp.t) : mpred :=
+    ∃ x, StdAtomicSpecs.owned_count_id_auth γ.(rec_gname) x. *)
 (*
     Definition rawR `{Σ : cpp_logic, σ : genv} (owner : option thread_idT) (count : nat) : Rep :=
       structR "std::recursive_mutex" 1$m **
       _field "MyRecursiveMutex::m_count" |-> ulonglongR 1$m count. *)
 
   Section with_Σ.
-    Context `{Σ : cpp_logic, σ : genv, !HasStdThreads Σ, !recursive_mutex.lockedG Σ}.
+    Context `{Σ : cpp_logic, σ : genv, !HasStdThreads Σ, !mutex.G Σ,
+      !StdAtomicSpecs.lockedG Σ}.
 
     Definition mutex_content (γ : gname) : Rep :=
       ∃ count,
@@ -70,15 +60,15 @@ Module custom_recursive_mutex.
         (this |-> mutex_content γ) **
       (* *)
       (this |-> mutex_content γ
-      (* ** recursive_mutex.token γ.(rec_gname) (* ? *) *)
+      (* ** std_recursive_mutex.token γ.(rec_gname) (* ? *) *)
       \\//
       exclusive_token γ.(excl_gname)
-      (* ** recursive_mutex.given_token γ.(rec_gname) (* ? *) *)
+      (* ** std_recursive_mutex.given_token γ.(rec_gname) (* ? *) *)
       ) **
       cinv lock_namespace γ.(cinv_gname) (∃ count owner,
         count_frag count **
         this ,, _field "MyRecursiveMutex::m_owner" |-> atomic_thread_idT 1$m owner **
-        recursive_mutex.owned_count_id_auth γ.(rec_gname) ((λ t, (t, Nat.pred count)) <$> owner) **
+        StdAtomicSpecs.owned_count_id_auth γ.(rec_gname) ((λ t, (t, Nat.pred count)) <$> owner) **
         [| owner = None <-> count = 0 |] **
         match count with
         | 0 => emp
