rocq-brick-libstdcpp/test/mutex/guard_recursive_cpp_proof.v
@@ -67,7 +67,7 @@ Succeed #[global] Instance: Inhabited TT := _.
 (** Canonical "constructor" for our telescope. *)
 Polymorphic Definition mk (a : Z) : TT :=
   {| tele_arg_head := a; tele_arg_tail := () |}.
-Succeed Definition b := recursive_mutex.Held 0 (mk 0).
+Succeed Definition b := std_recursive_mutex.Held 0 (mk 0).
 
 sl.lock
 Definition CR' `{Σ : cpp_logic, σ : genv} (a : Z) : Rep :=
@@ -82,13 +82,12 @@ Definition P `{Σ : cpp_logic, σ : genv} (this : ptr) : TT -t> mpred :=
 sl.lock
 Definition CR
   `{Σ : cpp_logic, σ : genv} {HAS_THREADS : HasStdThreads Σ}
-  `{!recursive_mutex.lockedG Σ}
-  `{!HasOwn (iPropI _) recursive_mutex.cmraR}
-  (γ : recursive_mutex.rmutex_gname) (q : cQp.t) :=
+  `{!std_recursive_mutex.G Σ}
+  (γ : std_recursive_mutex.gname) (q : cQp.t) :=
   structR "C" q **
-  _field "C::m" |-> recursive_mutex.derivedR γ q **
   as_Rep (fun this : ptr =>
-    recursive_mutex.inv_rmutex γ (∃ a : tele_arg TT, tele_app (P this) a)).
+    this ,, _field "C::m" |-> std_recursive_mutex.R γ q
+      (∃ a : tele_arg TT, tele_app (P this) a)).
 
 #[only(cfractional,ascfractional,cfracvalid,type_ptr)] derive CR.
 #[only(lazy_unfold(export))] derive CR.
@@ -96,10 +95,9 @@ Definition CR
 Section with_cpp.
   Context `{Σ : cpp_logic, σ : genv} {HAS_THREADS : HasStdThreads Σ}.
 
-  Context `{!recursive_mutex.lockedG Σ}.
-  Context `{!HasOwn (iPropI _) recursive_mutex.cmraR}.
+  Context `{!std_recursive_mutex.G Σ}.
 
-  #[local] Instance: `{WeaklyObjective1 (tele_app (P p))}.
+  #[local] Instance: `{Objective1 (tele_app (P p))}.
   Proof. Admitted.
 
   #[global] Instance P_timeless p a : Timeless (P p a).
@@ -115,15 +113,13 @@ Section with_cpp.
     \post[Vint 42] emp
   ).
 
-  Import recursive_mutex(lock_gname).
-
   cpp.spec "C::C()" from source as C_ctor_spec with (
     \this this
     \persist{thr} current_thread thr
     \post Exists γ,
       this |-> CR γ 1$m **
-      recursive_mutex.used_threads (lock_gname γ) {[thr]} **
-      recursive_mutex.acquireable (TT := TT) γ thr recursive_mutex.NotHeld (P this)
+      std_recursive_mutex.used_threads γ {[thr]} **
+      std_recursive_mutex.acquireable (TT := TT) γ thr std_recursive_mutex.NotHeld (P this)
   ).
 
   (** XXX Does not appear to help *)
@@ -138,9 +134,9 @@ Section with_cpp.
     rewrite {1}P.unlock.
     go.
 
-    iMod (recursive_mutex.use_thread thr (lock_gname t) ∅ with "[$]") as "?"; first set_solver; iModIntro.
+    iMod (std_recursive_mutex.use_thread_acquirable (TT := TT) thr t ∅ (P this) with "[$]") as "?"; first set_solver; iModIntro.
     go.
-    rewrite recursive_mutex.acquireable.unlock (left_id_L _ (∪)).
+    rewrite (left_id_L _ (∪)).
     go.
   Qed.
 
@@ -148,25 +144,23 @@ Section with_cpp.
     \this this
     \persist{thr} current_thread thr
     \pre{γ} this |-> CR γ 1$m
-    (* \pre recursive_mutex.used_threads (lock_gname γ) empty *)
-    \pre recursive_mutex.used_threads γ.(lock_gname) {[thr]}
-    \pre recursive_mutex.inv_rmutex γ (∃ xs, tele_app (TT := TT) (P this) xs)
-    \pre recursive_mutex.acquireable (TT := TT) γ thr recursive_mutex.NotHeld (P this)
+    (* \pre std_recursive_mutex.used_threads γ empty *)
+    \pre std_recursive_mutex.used_threads γ {[thr]}
+    \pre std_recursive_mutex.acquireable (TT := TT) γ thr std_recursive_mutex.NotHeld (P this)
     \post emp).
 
   Lemma C_dtor_ok :
-    (* We only get [|> recursive_mutex.dtor_spec'], and that's not enough *)
-    recursive_mutex.dtor_spec' |-- verify[source] "C::~C()".
+    (* We only get [|> std_recursive_mutex.std_dtor_spec], and that's not enough *)
+    std_recursive_mutex.std_dtor_spec |-- verify[source] "C::~C()".
   Proof.
     verify_shift; go.
-    wapply (recursive_mutex.logout thr _ ∅); first by set_solver.
-    rewrite recursive_mutex.acquireable.unlock /= (left_id_L _ (∪)).
+    wapply (std_recursive_mutex.logout_acquirable (TT := TT) thr _ ∅ (P this)); first by set_solver.
+    rewrite /= (left_id_L _ (∪)).
     go with br_erefl.
     iModIntro.
     go.
     progress destruct_tele; rewrite P.unlock /=.
     go.
-    iApply affine; [apply mpred_BiAffine|go].
   Qed.
 
   cpp.spec "C::one_answer()" from source inline.
@@ -181,18 +175,18 @@ Section with_cpp.
 
     iExists ?[K], (mk 42). go.
     iSplitL ""; [by go | go].
-    have [? [??]] : exists a, n = 1%nat /\ recursive_mutex.acquire a (recursive_mutex.release (recursive_mutex.Held n (mk 42))). {
+    have [? [??]] : exists a, n = 1%nat /\ std_recursive_mutex.acquire a (std_recursive_mutex.release (std_recursive_mutex.Held n (mk 42))). {
       lazymatch goal with
-      | _ : recursive_mutex.Held ?x _ = _ |- _ => rename x into n0
+      | _ : std_recursive_mutex.Held ?x _ = _ |- _ => rename x into n0
       end.
       (* This step breaks abstractions, but we have taken the lock yet hints don't
       give us access to the resouce. *)
       assert (n0 = 0 /\ n = 1)%nat as [-> ->]. {
-        rewrite-> recursive_mutex.release.unlock in *.
+        rewrite-> std_recursive_mutex.release.unlock in *.
         destruct n0, n; naive_solver.
       }
-      rewrite recursive_mutex.release.unlock /=.
-      exists recursive_mutex.NotHeld.
+      rewrite std_recursive_mutex.release.unlock /=.
+      exists std_recursive_mutex.NotHeld.
       split; first done.
       typeclasses eauto with br_hints.
     }
@@ -200,8 +194,8 @@ Section with_cpp.
     rewrite CR'.unlock.
     destruct args as [a1 []].
     go.
-    have [Ha1 Hrel]: (a1 = 42 /\ recursive_mutex.release (recursive_mutex.Held n (mk a1)) = recursive_mutex.NotHeld). {
-      rewrite-> recursive_mutex.release.unlock in *; naive_solver.
+    have [Ha1 Hrel]: (a1 = 42 /\ std_recursive_mutex.release (std_recursive_mutex.Held n (mk a1)) = std_recursive_mutex.NotHeld). {
+      rewrite-> std_recursive_mutex.release.unlock in *; naive_solver.
     }
     subst a1.
     iExists ?[K], (mk 42). rewrite Hrel /=.
