rocq-brick-libstdcpp/proof/mutex/spec/recursive_mutex_atomic.v
@@ -1,0 +1,542 @@
+Require Import iris.algebra.gset.
+Require Import iris.algebra.lib.excl_auth.
+
+Require Import skylabs.bi.tls_modalities.
+Require Import skylabs.bi.tls_modalities_rep.
+Require Import skylabs.bi.weakly_objective.
+Require Import skylabs.auto.cpp.weakly_local_with.
+
+Require Import skylabs.auto.cpp.proof.
+Require Import skylabs.brick.libstdcpp.mutex.spec.mutex.
+Require Export skylabs.brick.libstdcpp.runtime.pred.
+
+Require Import skylabs.brick.libstdcpp.mutex.requirements.
+Require Import skylabs.brick.libstdcpp.lib.lock_ghost.
+Require Import skylabs.brick.libstdcpp.mutex.inc_hpp.
+
+Require Export skylabs.brick.libstdcpp.mutex.spec.recursive_mutex.
+
+Import linearity.
+
+(** This file contains: 
+      - Atomic specs for recursive mutex [RecursiveMutexAtomicSpecs].
+      - An instantiation of (non-atomic) recursive mutex predicates
+        (which can be plugged into [recursive_mutex_spec]).
+      - A proof that the non-atomic specs refine the atomic version.
+*)
+
+(** Atomic specs for recursive mutex. *)
+Module RecursiveMutexAtomicSpecs (T : MutexCPPName).
+  (* FIXME the hardcoded strings can be derived from T.cpp_ty. *)
+
+  (* Not prodO thread_idTO natO. *)
+  (* at_specs thread that has zero, locked γ th 0 does not even know which thread has non-0. *)
+  Canonical Structure phys_stateUR := authR (optionR (exclR (prodO thread_idTO natO))).
+
+  (** <<locked γ th n>> <<th>> owns the mutex <<γ>> <<n>> times. *)
+  Class lockedG `{Σ : cpp_logic} := {
+    #[local] has_lock_ghost :: lock_ghost.lockG Σ;
+
+    #[local] has_phys_state :: HasOwn (iPropI _Σ) phys_stateUR;
+    #[local] has_phys_state_upd :: HasOwnUpd (iPropI _Σ) phys_stateUR;
+    #[local] has_phys_state_valid :: HasOwnValid (iPropI _Σ) phys_stateUR;
+    #[local] has_phys_state_unit :: HasOwnUnit mpredI phys_stateUR;
+  }.
+  #[global] Arguments lockedG {_ _} Σ : assert.
+
+  Record gname : Set := MkGname
+  { owned_count_id : iprop.gname;
+    locked_gname : iprop.gname;
+    inv_gname : iprop.gname;
+  }.
+
+  (** [owned_count_id_auth γ Some (th, n)] implies that the lock's count is [n + 1]. *)
+  sl.lock
+  Definition owned_count_id_auth `{Σ : cpp_logic, !lockedG Σ}
+    (γ : gname) (om : option (thread_idT * natO)) : mpred :=
+    own γ.(owned_count_id) (● (option_map Excl om)).
+  #[only(timeless)] derive owned_count_id_auth.
+
+  (** [owned_count_id_frag γ Some (th, n)] implies that the lock's count is [n + 1]. *)
+  sl.lock
+  Definition owned_count_id_frag `{Σ : cpp_logic, !lockedG Σ}
+    (γ : gname) (om : option (thread_idT * natO)) : mpred :=
+    own γ.(owned_count_id) (◯ (option_map Excl om)).
+  #[only(timeless)] derive owned_count_id_frag.
+
+  #[local] Open Scope nat_scope.
+
+  (** [locked γ th n] implies that the lock's count is [n]: see [used_threads]'s
+  definition and [owned_count_id_auth]'s informal contract. *)
+  sl.lock
+  Definition locked `{Σ : cpp_logic, !lockedG Σ}
+      (γ : gname) (th : thread_idT) (n : nat) : mpred :=
+    user γ.(locked_gname) th **
+    match n with
+    | 0 => owned_count_id_frag γ None
+    | S n => owned_count_id_frag γ (Some (th, n))
+    end.
+  #[only(timeless)] derive locked.
+
+  (* TODO: we should abstract this over the ownership that is produced and
+     then it can be used more generally. *)
+  sl.lock
+  Definition used_threads
+    `{Σ : cpp_logic, !lockedG Σ, !HasStdThreads Σ}
+    (γ : gname) (s : gset thread_idT) : mpred :=
+    lock_ghost.used_threads γ.(locked_gname) s.
+  #[only(timeless)] derive used_threads.
+
+  Section locked_with_cpp.
+    Context `{Σ : cpp_logic}.
+    Context `{!lockedG Σ}.
+    Context `{!HasStdThreads Σ}.
+
+    Lemma use_thread th g s :
+      th ∉ s ->
+      used_threads g s |--
+      (|==> used_threads g (s ∪ {[ th ]}) ** locked g th 0).
+    Proof.
+      rewrite used_threads.unlock locked.unlock owned_count_id_frag.unlock /=.
+      iIntros (Hni) "at_specs".
+      iMod (lock_ghost.login with "at_specs") as "[$ $]"; first done.
+      iApply own_unit.
+    Qed.
+
+    Lemma logout th g s :
+      th ∉ s ->
+      used_threads g (s ∪ {[ th ]}) ** locked g th 0 |--
+        (|==> used_threads g s ** owned_count_id_frag g None).
+    Proof.
+      rewrite used_threads.unlock locked.unlock.
+      iIntros (Hni) "(? & ? & $)".
+      iApply lock_ghost.logout; first done.
+      work.
+    Qed.
+
+    #[global] Instance owned_count_id_frag_WeaklyObjective γ om :
+      WeaklyObjective (PROP := iPropI _) (owned_count_id_frag γ om).
+    Proof. rewrite owned_count_id_frag.unlock. apply _. Qed.
+
+    #[global] Instance
+      locked_WeaklyObjective γ thr n :
+      WeaklyObjective (PROP := iPropI _) (locked γ thr n).
+    Proof. rewrite locked.unlock. apply _. Qed.
+
+    Lemma locked_excl_same_thread g th n m :
+      locked g th n ** locked g th m |-- False.
+    Proof.
+      rewrite locked.unlock.
+      work.
+      iDestruct (user_unique with "[$]") as "[]".
+    Qed.
+
+    Lemma locked_excl_different_thread g th th' n m :
+      locked g th n ** locked g th' m |-- [| n = 0 \/ m = 0 |] ** True.
+    Proof.
+      destruct (decide (th = th')) as [->|Hne]. {
+        rewrite locked_excl_same_thread. work.
+      }
+      rewrite locked.unlock.
+      iIntros "[[_ at_specs] [_ B]]".
+      destruct n, m; try auto. iExFalso.
+      rewrite owned_count_id_frag.unlock.
+      iDestruct (own_valid_2 with "at_specs B") as %HV; exfalso.
+      rewrite -auth_frag_op auth_frag_valid in HV.
+      done.
+    Qed.
+
+  End locked_with_cpp.
+
+(**
+Underlying pthread implementation for [PTHREAD_MUTEX_RECURSIVE_NP] case:
+
+  <<
+  /* Check whether we already hold the mutex.  */
+  if (mutex->__data.__owner == id)
+	{
+	  /* Just bump the counter.  */
+	  if (__glibc_unlikely (mutex->__data.__count + 1 == 0))
+	    /* Overflow of the counter.  */
+	    return EAGAIN;
+
+	  ++mutex->__data.__count;
+
+	  return 0;
+	}
+  (* LLL_MUTEX_LOCK_OPTIMIZED (mutex); *)
+  LLL_MUTEX_LOCK (mutex);
+  >>
+
+Informally, we can read mutex->__data.__owner atomically, and we know that
+mutex->__data.__owner == id if and only if our thread has completed locking the
+recursive mutex; hence, mutex->__data.__owner != id means that nobody is
+touching the mutex or other threads are operating on it, but at no point will they set __owner to our ID.
+
+Hence:
+1. [if (mutex->__data.__owner == id)], we can get sequential ownership of
+mutex->__data.__count, and of the underlying resources, and complete the lock operation.
+2. else, we can attempt to grab the underlying non-recursive lock, and be sure we
+  won't deadlock against ourselves.
+
+Formalizing step 1 seems nontrivial, but relatively routine.
+But the full pthread implementation would add annoying details.
+
+The right invariant might resemble the following, but significant details are TBD.
+[[
+cinv (
+  \exists x,
+  mutex->__data.__owner |-> x **
+  if bool_decide (x <> 0) then
+    (sequential ownership of count ** ownership of data protected by the lock) \/
+    some exclusive token (* needed to take the sequential out *)
+  else
+    emp
+  )
+]]
+*)
+  (* the mask of recursive_mutex *)
+  Definition mask := nroot .@@ "std" .@@ "recursive_mutex" .@@ "mask".
+
+  (** We base the implementation protocol on
+  https://github.com/bminor/glibc/blob/04e750e75b73957cf1c791535a3f4319534a52fc/nptl/pthread_mutex_lock.c#L90-L112.
+
+  official mirror:
+  https://sourceware.org/git/?p=glibc.git;a=blob;f=nptl/pthread_mutex_lock.c;h=a697f2b6ca8dfa9e4557ab3f44b87bc5ceeec014;hb=HEAD#l90
+  TODO: revise.
+  *)
+
+  (* NOTE: Invariant used to protect resource [r]
+
+      [[
+      inv (r \\// exists th n, locked th (S n))
+      ]]
+   *)
+
+
+  (** Intended meaning: ownership of physical C++ state for an instance of "std::recursive_mutex". *)
+  Parameter rawR : ∀ `{Σ : cpp_logic, σ : genv}, option thread_idT -> nat -> Rep.
+  (* The thread_idT is None (0) if there is no owner. *)
+  Axiom rawR_type_ptr : ∀ `{Σ : cpp_logic, σ : genv} o n,
+    Observe (type_ptrR T.cpp_ty) (rawR o n).
+  #[global] Existing Instance rawR_type_ptr.
+
+  Definition rmutex_N : namespace :=
+    nroot .@@ "std" .@@ "recursive_mutex" .@ "raw_inv".
+
+  (* recursive mutex -- ownership of the class. *)
+  sl.lock
+  Definition I `{Σ : cpp_logic, σ : genv, !lockedG Σ} (γ : gname) : Rep :=
+    type_ptrR T.cpp_ty **
+    cinv rmutex_N γ.(inv_gname) (∃ owner count, rawR owner count **
+      (* We use [Nat.pred] because [owned_count_id_auth] stores [counter - 1]. *)
+      pureR (owned_count_id_auth γ ((λ t, (t, Nat.pred count)) <$> owner))).
+  (* TODO: readd [|owner = None <-> count = O|] elsewhere, as sequential invariant in [R]. *)
+  #[only(knowledge (*,type_ptr="std::recursive_mutex"*) )] derive I.
+
+  sl.lock
+  Definition R `{Σ : cpp_logic, σ : genv, !lockedG Σ} (γ : gname) (q : cQp.t) : Rep :=
+    type_ptrR T.cpp_ty **
+    (* TODO: add here sequential ownership of the lock, and maybe replace I by the lock invariant.
+    Something like *)
+    (* _mutex_field |-> mutex.R q ... ** *)
+    pureR (cinv_own γ.(inv_gname) q).
+  #[only(cfracsplittable)] derive R.
+  #[global] Instance R_type_ptr `{Σ : cpp_logic, σ : genv, !lockedG Σ} γ q :
+    Observe (type_ptrR T.cpp_ty) (R γ q).
+  Proof. rewrite R.unlock. apply _. Qed.
+
+
+  Section base_construction.
+    Context `{Σ : cpp_logic} `{MOD : source ⊧ σ}.
+    Context {HAS_THREADS : HasStdThreads Σ}.
+    Context `{!lockedG Σ}.
+
+    #[global] Instance I_learn : Cbn (Learn (learn_eq ==> learn_hints.fin) I).
+    Proof. solve_learnable. Qed.
+    #[global] Instance R_learn : Cbn (Learn (learn_eq ==> any ==> learn_hints.fin) R).
+    Proof. solve_learnable. Qed.
+
+    Definition ctor_spec_body : ptr -> WpSpec mpred val val :=
+      (\this this
+      \post Exists g, this |-> R g 1$m ** used_threads g empty).
+
+    Definition dtor_spec_body : ptr -> WpSpec mpred val val :=
+      (\this this
+      \pre{g} this |-> R g 1$m
+      \pre used_threads g empty
+      \post emp).
+
+    Definition lock_spec_body : ptr -> WpSpec mpred val val :=
+      (\this this
+        \prepost{q g} this |-> R g q (* part of both pre and post *)
+        \persist{th} current_thread th
+        \pre{Q} AC << ∀ n , locked g th n >> @ top \ ↑ mask , empty
+                    << locked g th (S n) , COMM Q >>
+        \post Q).
+
+    Definition unlock_spec_body : ptr -> WpSpec mpred val val :=
+      (\this this
+        \prepost{q g} this |-> R g q (* part of both pre and post *)
+        \persist{th} current_thread th
+        \pre{Q} AC << ∀ n , locked g th (S n) >> @ top \ ↑ mask , empty
+                    << locked g th n , COMM Q >>
+        \post Q).
+
+  End base_construction.
+End RecursiveMutexAtomicSpecs.
+
+(** An instantiation of RecursiveMutexPreds. This is built on top of predicates
+    in RecursiveMutexAtomicSpecs, so the abstraction here is not ideal.
+    The main result here is that the atomic specs can derive the non-atomic 
+    ones; see the [RecursiveMutexRefinement] module defined later. *)
+Module RecursiveMutexPreds (T : MutexCPPName) <: RECURSIVE_MUTEX_PREDS T.
+  Module at_specs := RecursiveMutexAtomicSpecs T.
+  Include RecursiveMutexState.
+
+  Definition cpp_ty : type := T.cpp_ty.
+  #[global] Hint Opaque cpp_ty : sl_opacity.
+
+  Record rmutex_gname := MkGname
+    { lock_gname : at_specs.gname
+    ; level_gname : iprop.gname
+    ; cinv_gname : iprop.gname
+    }.
+  Definition gname := rmutex_gname.
+
+  Canonical Structure cmraR := excl_authR (prodO natO thread_idTO).
+
+  Class recursive_mutexG `{Σ : cpp_logic} := {
+    #[global] locked_G :: at_specs.lockedG Σ;
+    #[global] level_own :: HasOwn (iPropI _Σ) cmraR;
+  }.
+  Definition G := @recursive_mutexG.
+  Existing Class G.
+  #[global] Arguments G {_ _} Σ : assert.
+  #[global] Instance recursive_mutex_G `{Σ : cpp_logic} (H : G Σ) :
+    @recursive_mutexG _ _ Σ := H.
+
+  Definition rmutex_namespace :=
+    nroot .@@ "std" .@@ "recursive_mutex" .@@ "derived".
+
+  sl.lock
+  Definition inv_rmutex `{Σ : cpp_logic, !G Σ}
+      (g : gname) (P : mpred) : mpred :=
+    cinv rmutex_namespace g.(cinv_gname)
+      (Exists n th, own g.(level_gname) (●E (n, th)) **
+        match n with
+        | 0 => P ** own g.(level_gname) (◯E (n, th))
+        | S n => at_specs.locked g.(lock_gname) th (S n)
+        end).
+  #[only(knowledge)] derive inv_rmutex.
+
+  (** Fractional ownership of the physical recursive mutex and of the
+   cancellable invariant that protects the custom resource P.
+   The two fractions do not have to be the same, we just choose to make them
+   equal for convenience.
+  *)
+  sl.lock
+  Definition derivedR `{Σ : cpp_logic, σ : genv, !G Σ}
+      (g : gname) (q : cQp.t) : Rep :=
+    at_specs.R g.(lock_gname) q **
+    pureR (cinv_own g.(cinv_gname) q).
+  #[only(cfracsplittable)] derive derivedR.
+  #[global] Instance derivedR_type_ptr `{Σ : cpp_logic, σ : genv, !G Σ} g q :
+    Observe (type_ptrR cpp_ty) (derivedR g q).
+  Proof. rewrite derivedR.unlock /cpp_ty. apply _. Qed.
+
+  (** Public ownership packages the physical handle with its resource protocol. *)
+  Definition R `{Σ : cpp_logic, !G Σ} {HAS_THREADS : HasStdThreads Σ}
+      {σ : genv} (g : gname) (q : cQp.t) (P : mpred) : Rep :=
+    derivedR g q ** pureR (inv_rmutex g P).
+  #[global] Hint Opaque R : sl_opacity typeclass_instances.
+  #[only(cfractional,cfracvalid,ascfractional)] derive R.
+  #[global] Instance R_type_ptr `{Σ : cpp_logic, !G Σ}
+      {HAS_THREADS : HasStdThreads Σ} {σ : genv} g q P :
+    Observe (type_ptrR cpp_ty) (R g q P).
+  Proof. rewrite /R. apply _. Qed.
+
+  Definition used_threads `{Σ : cpp_logic, !G Σ, !HasStdThreads Σ}
+      (g : gname) (threads : gset thread_idT) : mpred :=
+    at_specs.used_threads g.(lock_gname) threads.
+  #[global] Hint Opaque used_threads : sl_opacity typeclass_instances.
+  #[only(timeless)] derive used_threads.
+
+  Definition held_token `{Σ : cpp_logic, !G Σ}
+      (g : gname) (th : thread_idT) (n : nat) : mpred :=
+    own g.(level_gname) (◯E (S n, th)).
+  #[global] Hint Opaque held_token : sl_opacity typeclass_instances.
+  #[only(timeless)] derive held_token.
+
+  Definition acquireable `{Σ : cpp_logic, !G Σ, !HasStdThreads Σ}
+      (g : gname) (th : thread_idT) {TT : tele} (t : acquire_state TT)
+      (P : TT -t> mpred) : mpred :=
+    current_thread th **
+    match t with
+    | NotHeld => at_specs.locked g.(lock_gname) th 0
+    | Held n args => held_token g th n ** tele_app P args
+    end.
+
+  #[global] Hint Opaque acquireable : sl_opacity typeclass_instances.
+
+  Section rules.
+    Context `{Σ : cpp_logic, !G Σ, !HasStdThreads Σ}.
+
+    Lemma acquireable_Held g th {TT : tele} n (args : TT) P :
+      acquireable g th (Held n args) P ⊣⊢
+        current_thread th ** held_token g th n ** tele_app P args.
+    Proof. rewrite /acquireable /=. done. Qed.
+
+    #[global] Instance acquireable_current_thread :
+      `{Observe (current_thread th) (acquireable g th (TT := TT) t P)}.
+    Proof. rewrite /acquireable; apply _. Qed.
+
+    Lemma use_thread_acquirable {TT} th g m P :
+      th ∉ m ->
+      current_thread th ** used_threads g m |-- (|==>
+        used_threads g (m ∪ {[th]}) ** acquireable (TT := TT) g th NotHeld P).
+    Proof.
+      rewrite /used_threads /acquireable /=.
+      work. wapply at_specs.use_thread; first done.
+      work with br_erefl. iModIntro; work.
+    Qed.
+
+    Lemma logout_acquirable {TT} th g m P :
+      th ∉ m ->
+      used_threads g (m ∪ {[th]}) ** acquireable (TT := TT) g th NotHeld P |--
+        (|==> used_threads g m).
+    Proof.
+      rewrite /used_threads /acquireable /=.
+      iIntros (Hnot) "[HU [_ HL]]".
+      iMod (at_specs.logout th g.(lock_gname) m Hnot
+        with "[$HU $HL]") as "(HU & Hunit)".
+      iModIntro.
+      iFrame "HU". iApply (affine with "Hunit"). apply mpred_BiAffine.
+    Qed.
+  End rules.
+End RecursiveMutexPreds.
+
+(** Atomic specs derive the non-atomic specs. *)
+Module RecursiveMutexRefinement (T : MutexCPPName).
+  Module Preds := RecursiveMutexPreds T.
+  Module Spec := recursive_mutex_spec T Preds.
+  Import Preds.
+
+Section with_cpp.
+  Context `{Σ : cpp_logic} `{MOD : source ⊧ σ}.
+  Context {HAS_THREADS : HasStdThreads Σ}.
+  Context `{!G Σ}.
+  Context `{HOV : !HasOwnValid mpredI cmraR, HOU : !HasOwnUpd mpredI cmraR}.
+
+  (* basically std_ctor_atomic_spec |-- std_ctor_non_atomic_spec *)
+  Lemma at_spec_impl_na_spec_ctor this :
+    elaborate.spec_entails_fupd
+      (Preds.at_specs.ctor_spec_body this)
+      (Spec.ctor_spec this).
+  Proof using MOD HOV HOU.
+    work.
+    iModIntro; work.
+    rewrite /acquireable /=.
+    iMod (own_alloc (●E (O, th) ⋅ ◯E (O, th))) as (g) "(? & ?)".
+    { apply excl_auth_valid. }
+    wname [Preds.at_specs.used_threads] "u".
+    wname [_ |-> _ _ _] "a".
+    iMod (cinv_alloc with "[-u a]") as (ginv) "(#Hinv & Hown)"; last first.
+    - iExists {| lock_gname := t; level_gname := g; cinv_gname:= ginv |}.
+      rewrite /R /used_threads _at_sep _at_pureR derivedR.unlock inv_rmutex.unlock /=.
+      iModIntro.
+      go with br_erefl $usenamed=true.
+    - ework with br_erefl.
+    - apply _.
+  Qed.
+
+  Lemma at_spec_impl_na_spec_dtor this :
+    elaborate.spec_entails_fupd
+      (Preds.at_specs.dtor_spec_body this)
+      (Spec.dtor_spec this).
+  Proof using MOD HOV HOU.
+    work.
+    rewrite /R /used_threads _at_sep _at_pureR derivedR.unlock inv_rmutex.unlock.
+    work.
+    iMod (cinv_cancel with "[$] [$]") as (n th) "(>? & ?)"; [done..|].
+
+    destruct n as [|n'] eqn:?; work; first last.
+    {
+      rewrite Preds.at_specs.locked.unlock /used_threads Preds.at_specs.used_threads.unlock.
+      wapply lock_ghost.used_threads_empty_no_not_locked; work with br_erefl.
+    }
+    iModIntro. work. iModIntro. ego with br_erefl.
+    (* _now_ we just need to leak ghost state and that's okay *)
+    wname [own] "L1"; wname [own] "L2"; iCombine "L1 L2" as "L".
+    iApply (affine with "L"). apply mpred_BiAffine.
+  Qed.
+
+  Lemma at_spec_impl_na_spec_lock this (xs : list val) (K : val -> mpred) :
+    Spec.lock_spec this xs K
+    |-- Preds.at_specs.lock_spec_body this xs K.
+  Proof using MOD HOV HOU.
+    revert xs K.
+    change (elaborate.spec_entails
+      (Preds.at_specs.lock_spec_body this)
+      (Spec.lock_spec this)).
+    work.
+    rewrite /R _at_sep _at_pureR derivedR.unlock; work.
+    iExists q, (cinv_own g.(cinv_gname) q **
+      (∃ t, [| acquire n t |] ∗ ▷ acquireable g th t P))%I.
+    wname [bi_wand] "W"; wfocus (bi_wand _ _) "W". { work $usenamed=true. }
+    rewrite inv_rmutex.unlock /acquireable /held_token.
+    work; iAcIntro; rewrite /commit_acc/=; work.
+    iInv rmutex_namespace as "[(%n' & %th' & >Hn & Hcases) ?]" "Hclose".
+    destruct n as [|n args]; simpl; [iExists 0 | iExists (S n)]; work.
+    2: iDestruct (own_valid_2 with "Hn [$]") as %[=]%excl_auth_agree_L; subst.
+    all: work $usenamed=true; iApply fupd_mask_intro; first set_solver;
+      iIntros "Hclose'"; work; iMod "Hclose'" as "_".
+    - destruct n'; first last. {
+        iMod "Hcases".
+        iDestruct (Preds.at_specs.locked_excl_different_thread with "[$]") as (?) "?".
+        exfalso. lia.
+      }
+      rewrite bi.later_sep bi.later_exist_except_0.
+      iDestruct "Hcases" as "(>(%args & ?) & >Hcase)".
+      iMod (own_update_2 with "Hn Hcase") as "(Hg & ?)";
+        first apply (excl_auth_update _ _ (1, th)).
+      wname [Preds.at_specs.locked _ th _] "Hlocked";
+        iMod ("Hclose" with "[$Hg $Hlocked //]") as "_"; iModIntro.
+      iExists (Held 0 args). work.
+    - iMod (own_update_2 with "Hn [$]") as "(Hg & ?)";
+        first apply (excl_auth_update _ _ (S (S n), th)).
+      wname [Preds.at_specs.locked _ th _] "Hlocked";
+        iMod ("Hclose" with "[$Hg $Hlocked //]") as "_"; iModIntro.
+      iExists (Held (S n) args). work.
+  Qed.
+
+  Lemma at_spec_impl_na_spec_unlock this (xs : list val) (K : val -> mpred) :
+    Spec.unlock_spec this xs K
+    |-- Preds.at_specs.unlock_spec_body this xs K.
+  Proof using MOD HOV HOU.
+    revert xs K.
+    change (elaborate.spec_entails
+      (Preds.at_specs.unlock_spec_body this)
+      (Spec.unlock_spec this)).
+    work.
+    rewrite /R _at_sep _at_pureR derivedR.unlock; work.
+    iExists q, (cinv_own g.(cinv_gname) q **
+      acquireable g th (release $ Held n args) P)%I.
+    wname [bi_wand] "W"; wfocus (bi_wand _ _) "W". { work $usenamed=true. }
+    rewrite inv_rmutex.unlock /acquireable /held_token.
+    work; iAcIntro; rewrite /commit_acc/=; work.
+    iInv rmutex_namespace as "[(%n' & %th' & >Hn & Hcases) ?]" "Hclose".
+    iDestruct (own_valid_2 with "Hn [$]") as %[=]%excl_auth_agree_L; subst.
+    iMod "Hcases".
+    iApply fupd_mask_intro; first set_solver; iIntros "Hclose'".
+    iExists n; work $usenamed=true.
+    iMod "Hclose'" as "_".
+    iMod (own_update_2 with "Hn [$]") as "(Hg & Hcase)";
+      first apply (excl_auth_update _ _ (n, th)).
+    rewrite release.unlock; destruct n; iFrame "#∗".
+    all: iMod ("Hclose" with "[-]") as "_";
+      ework $usenamed=true with br_erefl; done.
+  Qed.
+
+End with_cpp.
+End RecursiveMutexRefinement.
